rupicola/io/ExpRel.fst
@@ -297,11 +297,7 @@ let lem_equiv_prod' (g:typ_env) (#t:qType) (fs_e:fs_prod t) (e:closed_exp) :
 
 (** Rules **)
 
-open QExp (** just to use the helpers functions **)
-
-let equiv_unit g
-  : Lemma (helper_unit g `equiv_oval qUnit` EUnit)
-  =
+let equiv_unit g : Lemma (fs_oval_return g qUnit () ≈ EUnit) =
   introduce forall b (s:gsub g b) fsG h. fsG `(∽) h` s ==> qUnit ⦂ (h, (), gsubst s EUnit) with begin
     introduce _ ==> _ with _. begin
       assert (qUnit ∋ (h, (), EUnit));
@@ -309,9 +305,7 @@ let equiv_unit g
     end
   end
 
-let equiv_true g
-  : Lemma (helper_true g `equiv_oval qBool` ETrue)
-  =
+let equiv_true g : Lemma (fs_oval_return g qBool true ≈ ETrue) =
   introduce forall b (s:gsub g b) fsG h. fsG `(∽) h` s ==> qBool ⦂ (h, true, gsubst s ETrue) with begin
     introduce _ ==> _ with _. begin
       assert (qBool ∋ (h, true, ETrue));
@@ -319,9 +313,7 @@ let equiv_true g
     end
   end
 
-let equiv_false g
-  : Lemma (helper_false g `equiv_oval qBool` EFalse)
-  =
+let equiv_false g : Lemma (fs_oval_return g qBool false ≈ EFalse) =
   introduce forall b (s:gsub g b) fsG h. fsG `(∽) h` s ==> qBool ⦂ (h, false, gsubst s EFalse) with begin
     introduce _ ==> _ with _. begin
       assert (qBool ∋ (h, false, EFalse));
@@ -329,9 +321,7 @@ let equiv_false g
     end
   end
 
-let equiv_var g (x:var{Some? (g x)})
-  : Lemma ((fun (fsG:eval_env g) -> index fsG x) ≈ EVar x)
-  =
+let equiv_var g (x:var{Some? (g x)}) : Lemma (fs_oval_var g x ≈ EVar x) =
   introduce forall b (s:gsub g b) fsG h. fsG `(∽) h` s ==> Some?.v (g x) ⦂ (h, index fsG x, gsubst s (EVar x)) with begin
     introduce _ ==> _ with _. begin
       assert (Some?.v (g x) ∋ (h, index fsG x, s x));
@@ -339,9 +329,7 @@ let equiv_var g (x:var{Some? (g x)})
     end
   end
 
-let equiv_file_descr g fd
-  : Lemma (helper_file_descr g fd `equiv_oval qFileDescr` EFileDescr fd)
-  =
+let equiv_file_descr g fd : Lemma (fs_oval_return g qFileDescr fd ≈ EFileDescr fd) =
   introduce forall b (s:gsub g b) fsG h. fsG `(∽) h` s ==> qFileDescr ⦂ (h, fd, gsubst s (EFileDescr fd)) with begin
     introduce _ ==> _ with _. begin
       assert (qFileDescr ∋ (h, fd, (EFileDescr fd)));
@@ -350,9 +338,7 @@ let equiv_file_descr g fd
   end
 
 (** Used in compilation **)
-let equiv_var0 (g:typ_env) (t:qType)
-  : Lemma (helper_var0 g t ≈ EVar 0)
-  =
+let equiv_var0 (g:typ_env) (t:qType) : Lemma (fs_oval_var0 g t ≈ EVar 0) =
   introduce forall b (s:gsub (extend t g) b) fsG h. fsG `(∽) h` s ==>  t ⦂ (h, hd fsG, gsubst s (EVar 0)) with begin
     introduce _ ==> _ with _. begin
       index_0_hd fsG;
@@ -434,7 +420,7 @@ let rec shift_sub_equiv_sub_inc #t #g
 let equiv_varS (#g:typ_env) #a #t (s:fs_oval g a) (e:exp)
   : Lemma
       (requires (s ≈ e))
-      (ensures (helper_varS t s ≈ subst sub_inc e))
+      (ensures (fs_oval_varS t s ≈ subst sub_inc e))
   =
   lem_fv_in_env_varS g t e;
   introduce forall b (s':gsub (extend t g) b) (fsG:eval_env (extend t g)) (h:history). fsG `(∽) h` s' ==> a ⦂ (h, s (tail fsG), gsubst s' (subst sub_inc e)) with begin
@@ -504,7 +490,7 @@ let equiv_varS (#g:typ_env) #a #t (s:fs_oval g a) (e:exp)
 
 let equiv_lam #g (#t1:qType) (#t2:qType) (fs_body:fs_oval (extend t1 g) t2) (body:exp) : Lemma
   (requires fs_body ≈ body)
-  (ensures (helper_lambda fs_body ≈ ELam body)) =
+  (ensures (fs_oval_lambda fs_body ≈ ELam body)) =
   lem_fv_in_env_lam g t1 body;
   let g' = extend t1 g in
   let f : fs_oval g (t1 ^-> t2) = fun fsG x -> fs_body (stack fsG x) in
@@ -588,7 +574,7 @@ let equiv_app #g
   (e1:exp) (e2:exp)
   : Lemma
     (requires fs_e1 ≈ e1 /\ fs_e2 ≈ e2)
-    (ensures (helper_app fs_e1 fs_e2 ≈ EApp e1 e2)) =
+    (ensures fs_oval_app fs_e1 fs_e2 ≈ EApp e1 e2) =
   lem_fv_in_env_app g e1 e2;
   introduce forall b (s:gsub g b) fsG h. fsG `(∽) h` s ==> t2 ⦂ (h, (fs_e1 fsG) (fs_e2 fsG), gsubst s (EApp e1 e2)) with begin
     let fs_e1 = fs_e1 fsG in
@@ -636,7 +622,7 @@ let equiv_if #g
   (e1:exp) (e2:exp) (e3:exp)
   : Lemma
     (requires fs_e1 ≈ e1 /\ fs_e2 ≈ e2 /\ fs_e3 ≈ e3)
-    (ensures helper_if fs_e1 fs_e2 fs_e3 ≈ EIf e1 e2 e3) =
+    (ensures fs_oval_if fs_e1 fs_e2 fs_e3 ≈ EIf e1 e2 e3) =
   lem_fv_in_env_if g e1 e2 e3;
   introduce forall b (s:gsub g b) fsG h. fsG `(∽) h` s ==> t ⦂ (h, (if fs_e1 fsG then fs_e2 fsG else fs_e3 fsG), gsubst s (EIf e1 e2 e3)) with begin
     let fs_e1 = fs_e1 fsG in
@@ -686,7 +672,7 @@ let equiv_pair #g
   (e1:exp) (e2:exp)
   : Lemma
     (requires fs_e1 ≈ e1 /\ fs_e2 ≈ e2)
-    (ensures helper_pair fs_e1 fs_e2 ≈ EPair e1 e2) =
+    (ensures fs_oval_pair fs_e1 fs_e2 ≈ EPair e1 e2) =
   lem_fv_in_env_pair g e1 e2;
   let t = t1 ^* t2 in
   introduce forall b (s:gsub g b) fsG h. fsG `(∽) h` s ==>  t ⦂ (h, (fs_e1 fsG, fs_e2 fsG), gsubst s (EPair e1 e2)) with begin
@@ -739,7 +725,7 @@ let equiv_pair_fst_app #g
   (e12:exp)
   : Lemma
     (requires fs_e12 ≈ e12) (** is this too strict? we only care for the left to be equivalent. **)
-    (ensures helper_fst fs_e12 ≈ (EFst e12)) =
+    (ensures fs_oval_fmap fs_e12 fst ≈ (EFst e12)) =
   lem_fv_in_env_fst g e12;
   introduce forall b (s:gsub g b) fsG h. fsG `(∽) h` s ==>  t1 ⦂ (h, fst (fs_e12 fsG), gsubst s (EFst e12)) with begin
     let fs_e12 = fs_e12 fsG in
@@ -785,7 +771,7 @@ let equiv_pair_snd_steps #e #e' #h #lt #t1 #t2 #fs_e12 #fs_e #e12 (sq:squash (eq
 let equiv_pair_snd_app #g (#t1 #t2:qType) (fs_e12:fs_oval g (t1 ^* t2)) (e12:exp)
   : Lemma
     (requires fs_e12 ≈ e12) (** is this too strict? we only care for the left to be equivalent. **)
-    (ensures helper_snd fs_e12 ≈ (ESnd e12)) =
+    (ensures fs_oval_fmap fs_e12 snd ≈ (ESnd e12)) =
   lem_fv_in_env_snd g e12;
   introduce forall b (s:gsub g b) fsG h. fsG `(∽) h` s ==> t2 ⦂ (h, snd (fs_e12 fsG), gsubst s (ESnd e12)) with begin
     let fs_e12 = fs_e12 fsG in
@@ -823,7 +809,7 @@ let equiv_inl_steps #ex #ex' #h #lt #t1 #t2 #fs_e #fs_ex #e (sq:squash (equiv_in
 
 let equiv_inl #g (#t1 t2:qType) (fs_e:fs_oval g t1) (e:exp) : Lemma
   (requires fs_e ≈ e)
-  (ensures helper_inl t2 fs_e ≈ (EInl e)) =
+  (ensures fs_oval_fmap #g #t1 #(t1 ^+ t2) fs_e Inl ≈ (EInl e)) =
   lem_fv_in_env_inl g e;
   let t = t1 ^+ t2 in
   introduce forall b (s:gsub g b) fsG h. fsG `(∽) h` s ==> (t1 ^+ t2) ⦂ (h, Inl (fs_e fsG), gsubst s (EInl e)) with begin
@@ -862,7 +848,7 @@ let equiv_inr_steps #ex #ex' #h #lt #t1 #t2 #fs_e #fs_ex #e (sq:squash (equiv_in
 
 let equiv_inr #g (t1 #t2:qType) (fs_e:fs_oval g t2) (e:exp) : Lemma
   (requires fs_e ≈ e)
-  (ensures helper_inr t1 fs_e ≈ (EInr e)) =
+  (ensures fs_oval_fmap #g #t2 #(t1 ^+ t2) fs_e Inr ≈ (EInr e)) =
   lem_fv_in_env_inr g e;
   let t = t1 ^+ t2 in
   introduce forall b (s:gsub g b) fsG h. fsG `(∽) h` s ==> (t1 ^+ t2) ⦂ (h, Inr (fs_e fsG), gsubst s (EInr e)) with begin
@@ -929,7 +915,7 @@ let equiv_case
   (e_case e_lc e_rc:exp)
   : Lemma
     (requires fs_case ≈ e_case /\ fs_lc ≈ e_lc /\ fs_rc ≈ e_rc)
-    (ensures helper_case fs_case fs_lc fs_rc ≈ ECase e_case e_lc e_rc) =
+    (ensures fs_oval_case fs_case fs_lc fs_rc ≈ ECase e_case e_lc e_rc) =
   lem_fv_in_env_case g t1 t2 e_case e_lc e_rc;
   lem_fv_in_env_lam g t1 e_lc;
   lem_fv_in_env_lam g t2 e_rc;
@@ -972,7 +958,7 @@ let equiv_case
 let equiv_lam_prod #g (#t1:qType) (#t2:qType) (fs_body:fs_oprod (extend t1 g) t2) (body:exp)
   : Lemma
     (requires fs_body ≋ body)
-    (ensures helper_lambda_prod fs_body ≈ (ELam body)) =
+    (ensures fs_oval_lambda_oprod fs_body ≈ (ELam body)) =
   lem_fv_in_env_lam g t1 body;
   let g' = extend t1 g in
   let f : fs_oval g (t1 ^->!@ t2) = fun fsG x -> fs_body (stack fsG x) in
@@ -1012,7 +998,7 @@ let equiv_lam_prod #g (#t1:qType) (#t2:qType) (fs_body:fs_oprod (extend t1 g) t2
 let equiv_oprod_return #g (#t:qType) (fs_x:fs_oval g t) (x:exp)
   : Lemma
     (requires fs_x ≈ x)
-    (ensures helper_return_prod fs_x ≋ x) =
+    (ensures fs_oprod_return fs_x ≋ x) =
   introduce forall b (s:gsub g b) fsG h. fsG `(∽) h` s ==> t ⪾ (h, return (fs_x fsG), gsubst s x) with begin
     introduce _ ==> _ with _. begin
       let fs_x = fs_x fsG in
@@ -1063,7 +1049,7 @@ let equiv_bind_steps #e #e' #h #lt #a #b #fs_k' #fs_m #fs_e' #m #k' (sq:squash (
 let equiv_oprod_bind #g (#a #b:qType) (fs_m:fs_oprod g a) (fs_k:fs_oprod (extend a g) b) (m k:exp)
   : Lemma
     (requires fs_m ≋ m /\ fs_k ≋ k)
-    (ensures (helper_bind_prod fs_m fs_k) ≋ (EApp (ELam k) m)) =
+    (ensures (fs_oprod_bind fs_m fs_k) ≋ (EApp (ELam k) m)) =
   lem_fv_in_env_lam g a k;
   lem_fv_in_env_app g (ELam k) m;
   equiv_lam_prod fs_k k;
@@ -1118,7 +1104,7 @@ let equiv_oprod_app_steps #e #e' #h #lt #a #b #fs_f #fs_x #fs_e #f #x (sq:squash
 let equiv_oprod_app #g (#a #b:qType) (fs_f:fs_oval g (a ^->!@ b)) (fs_x:fs_oval g a) (f x:exp)
   : Lemma
     (requires fs_f ≈ f /\ fs_x ≈ x)
-    (ensures (helper_app_prod fs_f fs_x) ≋ (EApp f x)) =
+    (ensures (fs_oprod_app_oval_oval fs_f fs_x) ≋ (EApp f x)) =
   lem_fv_in_env_app g f x;
   introduce forall b' (s:gsub g b') fsG h. fsG `(∽) h` s ==> b ⪾ (h, (fs_f fsG) (fs_x fsG), gsubst s (EApp f x)) with begin
     let fs_f = fs_f fsG in
@@ -1138,6 +1124,14 @@ let equiv_oprod_app #g (#a #b:qType) (fs_f:fs_oval g (a ^->!@ b)) (fs_x:fs_oval 
       end
     end
   end
+
+let equiv_oprod_app' #g (#a #b:qType) (fs_f:fs_oprod g (a ^->!@ b)) (fs_x:fs_oprod g a) (f x:exp)
+  : Lemma
+    (requires fs_f ≋ f /\ fs_x ≋ x)
+    (ensures (fun fsG ->
+      let!@ f' = fs_f fsG in
+      let!@ x' = fs_x fsG in
+      f' x') ≋ (EApp f x)) = admit ()
 
 let equiv_if_prod_steps_pre (ex ex':closed_exp) (h:history) (lt:local_trace h) (a:qType) (fs_c:bool) (fs_t fs_e fs_ex:fs_prod a) (c t e:closed_exp) =
   (fs_ex == (if fs_c then fs_t else fs_e)) /\
@@ -1162,7 +1156,7 @@ let equiv_if_prod_steps #ex #ex' #h #lt #a #fs_c #fs_t #fs_e #fs_ex #c #t #e (sq
 let equiv_oprod_if #g (#a:qType) (fs_c:fs_oval g qBool) (fs_t fs_e:fs_oprod g a) (c t e:exp)
   : Lemma
     (requires fs_c ≈ c /\ fs_t ≋ t /\ fs_e ≋ e)
-    (ensures (helper_if_prod fs_c fs_t fs_e) ≋ (EIf c t e)) =
+    (ensures (fs_oprod_if_oval fs_c fs_t fs_e) ≋ (EIf c t e)) =
   lem_fv_in_env_if g c t e;
   introduce forall b' (s:gsub g b') fsG h. fsG `(∽) h` s ==> a ⪾ (h, (if (fs_c fsG) then (fs_t fsG) else (fs_e fsG)), gsubst s (EIf c t e)) with begin
     let fs_c = fs_c fsG in
@@ -1224,7 +1218,7 @@ let equiv_case_prod_steps #e #e' #h #lt #a #b #c #fs_cond #fs_inlc #fs_inrc #fs_
 let equiv_oprod_case #g (#a #b #c:qType) (fs_cond:fs_oval g (a ^+ b)) (fs_inlc:fs_oprod (extend a g) c) (fs_inrc:fs_oprod (extend b g) c) (cond inlc inrc:exp)
   : Lemma
     (requires fs_cond ≈ cond /\ fs_inlc ≋ inlc /\ fs_inrc ≋ inrc)
-    (ensures (helper_case_prod fs_cond fs_inlc fs_inrc) ≋ (ECase cond inlc inrc)) =
+    (ensures (fs_oprod_case_oval fs_cond fs_inlc fs_inrc) ≋ (ECase cond inlc inrc)) =
   lem_fv_in_env_case g a b cond inlc inrc;
   lem_fv_in_env_lam g a inlc;
   lem_fv_in_env_lam g b inrc;
@@ -1299,7 +1293,7 @@ let equiv_oprod_openfile_steps #e #e' #h #lt #fs_fnm #fs_e #fnm (sq:squash (equi
 let equiv_oprod_openfile #g (fs_fnm:fs_oval g qBool) (fnm:exp)
   : Lemma
     (requires fs_fnm ≈ fnm)
-    (ensures helper_prod_openfile fs_fnm ≋ EOpen fnm)
+    (ensures fs_oprod_openfile fs_fnm ≋ EOpen fnm)
   =
   lem_fv_in_env_openfile g fnm;
   introduce forall b (s:gsub g b) (fsG:eval_env g) (h:history). fsG `(∽) h` s ==> (qFileDescr ^+ qUnit) ⪾ (h, openfile (fs_fnm fsG), gsubst s (EOpen fnm)) with begin
@@ -1362,7 +1356,7 @@ let equiv_oprod_read_steps #e #e' #h #lt #fs_fd #fs_e #fd (sq:squash (equiv_opro
 let equiv_oprod_read #g (fs_fd:fs_oval g qFileDescr) (fd:exp)
   : Lemma
     (requires fs_fd ≈ fd)
-    (ensures helper_prod_read fs_fd ≋ ERead fd)
+    (ensures fs_oprod_read fs_fd ≋ ERead fd)
   =
   lem_fv_in_env_read g fd;
   introduce forall b (s:gsub g b) (fsG:eval_env g) (h:history). fsG `(∽) h` s ==> (qBool ^+ qUnit) ⪾ (h, read (fs_fd fsG), gsubst s (ERead fd)) with begin
@@ -1424,7 +1418,7 @@ let equiv_write_steps #e #e' #h #lt #fs_fd #fs_msg #fs_e #fd #msg (sq:squash (eq
 let equiv_oprod_write #g (fs_fd:fs_oval g qFileDescr) (fs_msg:fs_oval g qBool) (fd msg:exp)
   : Lemma
     (requires fs_fd ≈ fd /\ fs_msg ≈ msg)
-    (ensures helper_prod_write fs_fd fs_msg ≋ EWrite fd msg)
+    (ensures fs_oprod_write fs_fd fs_msg ≋ EWrite fd msg)
   =
   lem_fv_in_env_write g fd msg;
   introduce forall b (s:gsub g b) (fsG:eval_env g) (h:history). fsG `(∽) h` s ==> (qUnit ^+ qUnit) ⪾ (h, write (fs_fd fsG, fs_msg fsG), gsubst s (EWrite fd msg)) with begin
@@ -1481,7 +1475,7 @@ let equiv_oprod_close_steps #e #e' #h #lt #fs_fd #fs_e #fd (sq:squash (equiv_opr
 let equiv_oprod_close #g (fs_fd:fs_oval g qFileDescr) (fd:exp)
   : Lemma
     (requires fs_fd ≈ fd)
-    (ensures helper_prod_close fs_fd ≋ EClose fd)
+    (ensures fs_oprod_close fs_fd ≋ EClose fd)
   =
   lem_fv_in_env_close g fd;
   introduce forall b (s:gsub g b) (fsG:eval_env g) (h:history). fsG `(∽) h` s ==> (qUnit ^+ qUnit) ⪾ (h, close (fs_fd fsG), gsubst s (EClose fd)) with begin
@@ -1500,4 +1494,3 @@ let equiv_oprod_close #g (fs_fd:fs_oval g qFileDescr) (fd:exp)
       end
     end
   end
- 
