rupicola/io/IO.fsti
@@ -16,6 +16,8 @@ val io (a:Type u#a) : Type u#a
 
 val io_return (#a:Type) (x:a) : io a
 
+val extract_v_from_io_return (#a:Type) (m:(io a){exists x. m == io_return x}) : (x:a{io_return x == m})
+
 val io_bind
   (#a:Type u#a)
   (#b:Type u#b)
